Revert "Extraction"
This reverts commit 2c35db92fdbbfa7c15f035ceed5a34d2e8836c5e.

debug/Debug.mli
@@ -16,6 +16,7 @@ open DwarfTypes
 open BinNums
 open Sections
 
+
 (* Record used for storing references to the actual implementation functions *)
 type implem =
     {
