common/Events.v
@@ -286,9 +286,9 @@ Inductive eventval_match: eventval -> typ -> atom -> Prop :=
       eventval_match (EVfloat f t) Tfloat (Vfloat f, t)
   | ev_match_single: forall f t,
       eventval_match (EVsingle f t) Tsingle (Vsingle f, t)
-  | ev_match_ptr: forall id b base bound ofs t,
+  | ev_match_ptr: forall id b ofs t,
       public_symbol ge id = true ->
-      find_symbol ge id = Some (b,base,bound,t) ->
+      find_symbol ge id = Some (b,t) ->
       eventval_match (EVptr_global id ofs t) Tptr (Vptr b ofs, t).
 
 Inductive eventval_list_match: list eventval -> list typ -> list atom -> Prop :=
@@ -342,11 +342,10 @@ Qed.
 
 Lemma eventval_match_determ_2:
   forall ev1 ev2 ty v, eventval_match ev1 ty v -> eventval_match ev2 ty v -> ev1 = ev2.
-Admitted.
-(*Proof.
+Proof.
   intros. inv H; inv H0; auto.
-  decEq. unfold find_symbol in *. eapply genv_vars_inj; eauto.
-Qed.*)
+  decEq. eapply genv_vars_inj; eauto.
+Qed.
 
 Lemma eventval_list_match_determ_2:
   forall evl1 tyl vl, eventval_list_match evl1 tyl vl ->
@@ -441,13 +440,12 @@ Hypothesis symbols_preserved:
 
 Lemma eventval_match_preserved:
   forall ev ty v,
-    eventval_match ge1 ev ty v -> eventval_match ge2 ev ty v.
-Admitted.
-(*Proof.
+  eventval_match ge1 ev ty v -> eventval_match ge2 ev ty v.
+Proof.
   induction 1; constructor; auto.
   rewrite public_preserved; auto.
   rewrite symbols_preserved; auto.
-Qed.*)
+Qed.
 
 Lemma eventval_list_match_preserved:
   forall evl tyl vl,
@@ -460,7 +458,7 @@ End EVENTVAL_INV.
 
 (** Compatibility with memory injections *)
 
-(*Section EVENTVAL_INJECT.
+Section EVENTVAL_INJECT.
 
   Variable F: Type.
   Variable V: Type.
@@ -512,7 +510,7 @@ Admitted.
   inv H1. constructor. eapply eventval_match_inject; eauto. eauto.
 Qed.*)
 
-End EVENTVAL_INJECT.*)
+End EVENTVAL_INJECT.
 
 (** * Matching traces. *)
 
@@ -584,28 +582,28 @@ Fixpoint output_trace (t: trace) : Prop :=
 
 Inductive volatile_load (ge: Genv.t F V):
                    memory_chunk -> mem -> block -> ptrofs -> trace -> atom -> list tag -> Prop :=
-  | volatile_load_vol: forall chunk m base block pt ofs id ev v vt,
+  | volatile_load_vol: forall chunk m pt ofs id ev v vt lts,
       addr_is_volatile ge ofs = true ->
-      find_symbol ge id = Some (dummy,base,block,pt) ->
+      find_symbol ge id = Some (dummy,pt) ->
       eventval_match ge ev (type_of_chunk chunk) (v,vt) ->
       volatile_load ge chunk m dummy ofs
-                    (Event_vload chunk id ofs ev :: nil)
-                    (Val.load_result chunk v,vt)
-                    (load_ltags chunk m dummy (Ptrofs.unsigned ofs))
-  | volatile_load_nonvol: forall chunk m ofs v,
+                      (Event_vload chunk id ofs ev :: nil)
+                      (Val.load_result chunk v,vt)
+                      lts
+  | volatile_load_nonvol: forall chunk m ofs v lts,
       addr_is_volatile ge ofs = false ->
       Mem.load chunk m dummy (Ptrofs.unsigned ofs) = Some v ->
-      volatile_load ge chunk m dummy ofs E0 v (load_ltags chunk m dummy (Ptrofs.unsigned ofs))
-  | volatile_load_block: forall chunk m b ofs v,
+      volatile_load ge chunk m dummy ofs E0 v lts
+  | volatile_load_block: forall chunk m b ofs v lts,
       b <> dummy ->
       Mem.load chunk m b (Ptrofs.unsigned ofs) = Some v ->
-      volatile_load ge chunk m b ofs E0 v (load_ltags chunk m b (Ptrofs.unsigned ofs)).
+      volatile_load ge chunk m b ofs E0 v lts.
 
 Inductive volatile_store (ge: Genv.t F V):
                   memory_chunk -> mem -> block -> ptrofs -> atom -> list tag -> trace -> mem -> Prop :=
-  | volatile_store_vol: forall chunk m base block pt ofs id ev v vt lts,
+  | volatile_store_vol: forall chunk m pt ofs id ev v vt lts,
       Genv.addr_is_volatile ge ofs = true ->
-      Genv.find_symbol ge id = Some (dummy,base,block,pt) ->
+      Genv.find_symbol ge id = Some (dummy,pt) ->
       eventval_match ge ev (type_of_chunk chunk) (Val.load_result chunk v, vt) ->
       volatile_store ge chunk m dummy ofs (v,vt) lts
                      (Event_vstore chunk id ofs ev :: nil)
@@ -653,7 +651,7 @@ Definition inject_separated (f f': meminj) (m1 m2: mem): Prop :=
   f b1 = None -> f' b1 = Some(b2, delta) ->
   ~Mem.valid_block m1 b1 /\ ~Mem.valid_block m2 b2.*)
 
-(*Record extcall_properties (sem: extcall_sem) (sg: signature) : Prop :=
+Record extcall_properties (sem: extcall_sem) (sg: signature) : Prop :=
   mk_extcall_properties {
 
 (** The return value of an external call must agree with its signature. *)
@@ -722,7 +720,7 @@ Definition inject_separated (f f': meminj) (m1 m2: mem): Prop :=
     forall ge vargs m t1 vres1 m1 t2 vres2 m2,
     sem ge vargs m t1 vres1 m1 -> sem ge vargs m t2 vres2 m2 ->
     match_traces ge t1 t2 /\ (t1 = t2 -> vres1 = vres2 /\ m1 = m2)
-}.*)
+}.
 
 (** ** Semantics of volatile loads *)
 
@@ -733,12 +731,13 @@ Inductive volatile_load_sem (chunk: memory_chunk) (ge: Genv.t F V):
       (*TODO: check tags *)
       volatile_load_sem chunk ge ((Vptr b ofs, pt) :: nil) m t (v,vt) m.
 
-(*Lemma volatile_load_preserved:
+Lemma volatile_load_preserved:
   forall ge1 ge2 chunk m b ofs t v vt lts,
   Genv.equiv ge1 ge2 ->
   volatile_load ge1 chunk m b ofs t (v, vt) lts ->
   volatile_load ge2 chunk m b ofs t (v, vt) lts.
-Proof.
+Admitted.
+(*Proof.
   intros. destruct H as (A & B & C). inv H0; constructor; auto.
   rewrite C; auto.
   rewrite A; auto.
@@ -793,11 +792,12 @@ Admitted.
   exists v1; constructor; auto.
 Qed.*)
 
-(*Lemma volatile_load_ok:
+Lemma volatile_load_ok:
   forall chunk,
-    extcall_properties (volatile_load_sem chunk)
-                       (mksignature (Tptr :: nil) (rettype_of_chunk chunk) cc_default).
-Proof.
+  extcall_properties (volatile_load_sem chunk)
+                     (mksignature (Tptr :: nil) (rettype_of_chunk chunk) cc_default).
+Admitted.
+(*Proof.
   intros; constructor; intros.
 (* well typed *)
 - inv H. inv H0. apply Val.load_result_rettype.
@@ -842,12 +842,13 @@ Inductive volatile_store_sem (chunk: memory_chunk) (ge: Genv.t F V):
       (* TODO: check tags *)
       volatile_store_sem chunk ge ((Vptr b ofs,pt) :: (v,vt) :: nil) m1 t (Vundef,def_tag) m2.
 
-(*Lemma volatile_store_preserved:
+Lemma volatile_store_preserved:
   forall ge1 ge2 chunk m1 b ofs v lts t m2,
   Genv.equiv ge1 ge2 ->
   volatile_store ge1 chunk m1 b ofs v lts t m2 ->
   volatile_store ge2 chunk m1 b ofs v lts t m2.
-Proof.
+Admitted.
+(*Proof.
   intros. destruct H as (A & B & C). inv H0; constructor; auto.
   rewrite C; auto.
   rewrite A; auto.
@@ -954,11 +955,12 @@ Proof.
   intros. inv H; inv H0; auto.
 Qed.
 
-(*Lemma volatile_store_ok:
+Lemma volatile_store_ok:
   forall chunk,
   extcall_properties (volatile_store_sem chunk)
                      (mksignature (Tptr :: type_of_chunk chunk :: nil) Tvoid cc_default).
-Proof.
+Admitted.
+(*Proof.
   intros; constructor; intros.
 (* well typed *)
 - unfold proj_sig_res; simpl. inv H; constructor.
@@ -997,10 +999,11 @@ Inductive extcall_malloc_sem (ge: Genv.t F V):
     Mem.store Mptr m' Mem.dummy (- size_chunk Mptr) (Vptrofs sz, vt) lts = Some m'' ->
     extcall_malloc_sem ge ((Vptrofs sz,st) :: nil) m E0 (Vptr Mem.dummy (Ptrofs.repr lo), pt) m''.
 
-(*Lemma extcall_malloc_ok:
+Lemma extcall_malloc_ok:
   extcall_properties extcall_malloc_sem
                      (mksignature (Tptr :: nil) Tptr cc_default).
-Proof.
+Admitted.
+(*Proof.
   assert (UNCHANGED:
     forall (P: block -> Z -> Prop) m lo hi v m' b m'',
     Mem.alloc m lo hi = (m', b) ->
@@ -1086,10 +1089,11 @@ Inductive extcall_free_sem (ge: Genv.t F V):
 | extcall_free_sem_null: forall m pt,
     extcall_free_sem ge ((Vnullptr,pt) :: nil) m E0 (Vundef,def_tag) m.
 
-(*Lemma extcall_free_ok:
+Lemma extcall_free_ok:
   extcall_properties extcall_free_sem
                      (mksignature (Tptr :: nil) Tvoid cc_default).
-Proof.
+Admitted.
+(*Proof.
   constructor; intros.
 (* well typed *)
 - inv H; simpl; auto.
@@ -1185,11 +1189,12 @@ Inductive extcall_memcpy_sem (sz al: Z) (ge: Genv.t F V):
       Mem.storebytes m Mem.dummy (Ptrofs.unsigned odst) bytes lts = Some m' ->
       extcall_memcpy_sem sz al ge ((Vptr Mem.dummy odst,pt1) :: (Vptr Mem.dummy osrc,pt2) :: nil) m E0 (Vundef,def_tag) m'.
 
-(*Lemma extcall_memcpy_ok:
+Lemma extcall_memcpy_ok:
   forall sz al,
   extcall_properties (extcall_memcpy_sem sz al)
                      (mksignature (Tptr :: Tptr :: nil) Tvoid cc_default).
-Proof.
+Admitted.
+(*Proof.
   intros. constructor.
 - (* return type *)
   intros. inv H. exact I.
@@ -1290,7 +1295,7 @@ Inductive extcall_annot_sem (text: string) (targs: list typ) (ge: Genv.t F V):
       eventval_list_match ge args targs vargs ->
       extcall_annot_sem text targs ge vargs m (Event_annot text args :: E0) (Vundef,def_tag) m.
 
-(*Lemma extcall_annot_ok:
+Lemma extcall_annot_ok:
   forall text targs,
   extcall_properties (extcall_annot_sem text targs)
                      (mksignature targs Tvoid cc_default).
@@ -1323,7 +1328,7 @@ Proof.
 - inv H; inv H0.
   assert (args = args0). eapply eventval_list_match_determ_2; eauto. subst args0.
   split. constructor. auto.
-Qed.*)
+Qed.
 
 Inductive extcall_annot_val_sem (text: string) (targ: typ) (ge: Genv.t F V):
               list atom -> mem -> trace -> atom -> mem -> Prop :=
@@ -1331,7 +1336,7 @@ Inductive extcall_annot_val_sem (text: string) (targ: typ) (ge: Genv.t F V):
       eventval_match ge arg targ varg ->
       extcall_annot_val_sem text targ ge (varg :: nil) m (Event_annot text (arg :: nil) :: E0) varg m.
 
-(*Lemma extcall_annot_val_ok:
+Lemma extcall_annot_val_ok:
   forall text targ,
   extcall_properties (extcall_annot_val_sem text targ)
                      (mksignature (targ :: nil) targ cc_default).
@@ -1364,14 +1369,14 @@ Proof.
 - inv H; inv H0.
   assert (arg = arg0). eapply eventval_match_determ_2; eauto. subst arg0.
   split. constructor. auto.
-Qed.*)
+Qed.
 
 Inductive extcall_debug_sem (ge: Genv.t F V):
               list atom -> mem -> trace -> atom -> mem -> Prop :=
   | extcall_debug_sem_intro: forall vargs m,
       extcall_debug_sem ge vargs m E0 (Vundef,def_tag) m.
 
-(*Lemma extcall_debug_ok:
+Lemma extcall_debug_ok:
   forall targs,
   extcall_properties extcall_debug_sem
                      (mksignature targs Tvoid cc_default).
@@ -1399,7 +1404,7 @@ Proof.
 (* determ *)
 - inv H; inv H0.
   split. constructor. auto.
-Qed.*)
+Qed.
 
 (** ** Semantics of known built-in functions. *)
 
@@ -1413,9 +1418,10 @@ Inductive known_builtin_sem (bf: builtin_function) (ge: Genv.t F V):
       builtin_function_sem bf vargs = Some vres ->
       known_builtin_sem bf ge (map (fun v => (v,def_tag)) vargs) m E0 (vres,def_tag) m.
 
-(*Lemma known_builtin_ok: forall bf,
+Lemma known_builtin_ok: forall bf,
   extcall_properties (known_builtin_sem bf) (builtin_function_sig bf).
-Proof.
+Admitted.
+(*Proof.
   intros. set (bsem := builtin_function_sem bf). constructor; intros.
 (* well typed *)
 - inv H.
@@ -1462,15 +1468,15 @@ Qed.*)
 
 Parameter external_functions_sem: String.string -> signature -> extcall_sem.
 
-(*Axiom external_functions_properties:
-  forall id sg, extcall_properties (external_functions_sem id sg) sg.*)
+Axiom external_functions_properties:
+  forall id sg, extcall_properties (external_functions_sem id sg) sg.
 
 (** We treat inline assembly similarly. *)
 
 Parameter inline_assembly_sem: String.string -> signature -> extcall_sem.
 
-(*Axiom inline_assembly_properties:
-  forall id sg, extcall_properties (inline_assembly_sem id sg) sg.*)
+Axiom inline_assembly_properties:
+  forall id sg, extcall_properties (inline_assembly_sem id sg) sg.
 
 (** ** Combined semantics of external calls *)
 
@@ -1480,7 +1486,7 @@ Definition builtin_or_external_sem name sg :=
   | None => external_functions_sem name sg
   end.
 
-(*Lemma builtin_or_external_sem_ok: forall name sg,
+Lemma builtin_or_external_sem_ok: forall name sg,
   extcall_properties (builtin_or_external_sem name sg) sg.
 Proof.
   unfold builtin_or_external_sem; intros. 
@@ -1488,7 +1494,7 @@ Proof.
 - exploit lookup_builtin_function_sig; eauto. intros EQ; subst sg.
   apply known_builtin_ok.
 - apply external_functions_properties.
-Qed.*)
+Qed.
 
 (** Combining the semantics given above for the various kinds of external calls,
   we define the predicate [external_call] that relates:
@@ -1517,7 +1523,7 @@ Definition external_call (ef: external_function): extcall_sem :=
   | EF_debug kind txt targs => extcall_debug_sem
   end.
 
-(*Theorem external_call_spec:
+Theorem external_call_spec:
   forall ef,
   extcall_properties (external_call ef) (ef_sig ef).
 Proof.
@@ -1534,18 +1540,18 @@ Proof.
   apply extcall_annot_val_ok.
   apply inline_assembly_properties.
   apply extcall_debug_ok.
-Qed.*)
+Qed.
 
-(*Definition external_call_well_typed_gen ef := ec_well_typed (external_call_spec ef).
+Definition external_call_well_typed_gen ef := ec_well_typed (external_call_spec ef).
 Definition external_call_symbols_preserved ef := ec_symbols_preserved (external_call_spec ef).
 Definition external_call_valid_block ef := ec_valid_block (external_call_spec ef).
-Definition external_call_max_perm ef := ec_max_perm (external_call_spec ef).
+(*Definition external_call_max_perm ef := ec_max_perm (external_call_spec ef).
 Definition external_call_readonly ef := ec_readonly (external_call_spec ef).
 Definition external_call_mem_extends ef := ec_mem_extends (external_call_spec ef).
-Definition external_call_mem_inject_gen ef := ec_mem_inject (external_call_spec ef).
+Definition external_call_mem_inject_gen ef := ec_mem_inject (external_call_spec ef).*)
 Definition external_call_trace_length ef := ec_trace_length (external_call_spec ef).
 Definition external_call_receptive ef := ec_receptive (external_call_spec ef).
-Definition external_call_determ ef := ec_determ (external_call_spec ef).*)
+Definition external_call_determ ef := ec_determ (external_call_spec ef).
 
 (** Corollary of [external_call_well_typed_gen]. *)
 
@@ -1553,10 +1559,9 @@ Lemma external_call_well_typed:
   forall ef ge vargs m1 t vres m2,
   external_call ef ge vargs m1 t vres m2 ->
   Val.has_type (fst vres) (proj_sig_res (ef_sig ef)).
-Admitted.
-(*Proof.
+Proof.
   intros. apply Val.has_proj_rettype. eapply external_call_well_typed_gen; eauto.
-Qed.*)
+Qed.
 
 (** Special case of [external_call_mem_inject_gen] (for backward compatibility) *)
 
@@ -1599,20 +1604,18 @@ Lemma external_call_match_traces:
   external_call ef ge vargs m t1 vres1 m1 ->
   external_call ef ge vargs m t2 vres2 m2 ->
   match_traces ge t1 t2.
-Admitted.
-(*Proof.
+Proof.
   intros. exploit external_call_determ. eexact H. eexact H0. tauto.
-Qed.*)
+Qed.
 
 Lemma external_call_deterministic:
   forall ef ge vargs m t vres1 m1 vres2 m2,
   external_call ef ge vargs m t vres1 m1 ->
   external_call ef ge vargs m t vres2 m2 ->
   vres1 = vres2 /\ m1 = m2.
-Admitted.
-(*Proof.
+Proof.
   intros. exploit external_call_determ. eexact H. eexact H0. intuition.
-Qed.*)
+Qed.
 
 End OUTPUT_EVENTS.
 
